\documentclass[12pt,letterpaper]{article}
\usepackage[utf8]{inputenc}
\usepackage{amsmath}
\usepackage{amsfonts}
\usepackage{amssymb}
\usepackage{graphicx}
\usepackage{lastpage}
\usepackage[left=1.00in, right=1.00in, top=1.00in, bottom=1.00in]{geometry}
\usepackage{fancyhdr}
\title{Math 523 HW 6}
\author{Morgan Gribbins}
\date{}
\pagestyle{fancy}
\fancyhf{}
\lhead{Page \thepage\ of \pageref{LastPage}}
\begin{document}
	
\maketitle

\section*{Section 2.4}

In Exercises 2 to 8, give the order of each of the zeros of the given function.

\textbf{(2)} \((e^{z}-1)^{2}\) \\

This function has zeros at \(z = 2\pi k\), \(k \in \mathbb{Z}\), each with order 2, as the first derivative is \(0\) at these zeros, and the 2nd derivative does not yield zero. \\

\textbf{(4)} \((z^{2}-4z+4)^{3}\) \\

This function has its only zero at \(z=2\), which has order 6.\\

\textbf{(6)} \(\log (1- z),\ |z| < 1\) \\

This function has its only zero at \(z=0\), and this has order 1.\\

\textbf{(8)} \(\frac{z}{z^{2}+1}\) \\

This function has its only zero at \(z=0\), and this has order 1.\\

In Exercises 10 and 12, find the power-series expansion about the given point for each of the functions; find the largest disc in which the series is valid.

\textbf{(10)} \(e^{z}\) about \(z_{0} = \pi i\) \\

\[e^{z} = \sum_{n=0}^{\infty} (z-\pi i)^{n}/n!,\] which is entire. \\

\textbf{(12)} \(\frac{(z^{2}}{1-z}\) about \(z_{0} = 0\) \\

\[\frac{z^{2}}{1-z} = \sum_{n=0}^{\infty} z^{n+2},\] which is valid within the disc \(|z| < 1\). \\

\textbf{(25)} Find all solutions to the differential equation \[f''(z) + \beta^{2}f(z) = 0,\ f \text{ is an entire function.}\] \\

Let \(f(z) = \sum_{n=0}^{\infty} a_{n}z^{n}\). The differential equation is then \[\sum_{n=2}^{\infty} a_{n}(n^{2} -n)z^{n-2} +\beta^{2}\sum_{n=0}^{\infty} a_{n}z^{n} = 0\] \[\implies (\beta^{2}a_{0} + 2a_{2}) + z(\beta^{2}a_{1} + 6a_{3}) + z^{2}(\beta^{2}a_{2} + 12a_{4}) + z^{3}(\beta^{2}a_{3} + 20a_{5}) + ... = 0 \] \[\implies \sum_{n = 0}^{\infty} (\beta^{2}a_{n} + (n^{2} + 3n + 2)a_{n+2})z^{n} = 0\] \[\implies \beta^{2}a_{n} = (-n^{2} - 3n - 2)a_{n+2} \implies a_{2} = -\beta^{2}a_{0}/2,\ a_{3} = -\beta^{2}a_{1}/6,\] and the rest of the terms are recursively provided by this rule. \\

\textbf{(26)} Use the technique of Exercise 25 to give the solutions of these differential equations:

\textbf{(26a)} \(f''(z) -3f'(z) +2f(z) = 0;\ a_{0} = 1,\ a_{1} = 2.\) \\

Let \(f(z) = \sum_{n=0}^{\infty} a_{n}z^{n}\). This equation is then \[\sum_{n=2}^{\infty} (n^{2}-n)a_{n}z^{n-2} - \sum_{n=1}^{\infty} 3na_{n}z^{n-1} + \sum_{n=0}^{\infty}2a_{n}z^{n} = 0\] \[\implies (2a_{0}-3a_{1}+2a_{2})+z(2a_{1} -6a_{2} + 6a_{3})+z^{2}(2a_{2} - 9a_{3} + 12a_{4})+z^{3}(2a_{3} - 12a_{4} + 20a_{5}) + ... = 0.\] This means that \[2a_{n} - 3(n+1)a_{n+1} + (n^{2} + 3n + 2)a_{n+2} = 0.\] With \(a_{0} = 1\) and \(a_{1} = 2\), the rest of these terms may be recursively solved. \\

\textbf{(26c)} \(f''(z) + 2f'(z) + f(z) = 0;\ a_{0} = 0,\ a_{1} = 1.\) \\

Let \(f(z) = \sum_{n=0}^{\infty} a_{n}z^{n}\). This equation is then \[\sum_{n=2}^{\infty} (n^{2}-n)a_{n}z^{n-2} + \sum_{n=1}^{\infty} 2na_{n}z^{n-1} + \sum_{n=0}^{\infty}a_{n}z^{n} = 0\] \[\implies (a_{0}+2a_{1}+2a_{2})+z(a_{1} +4a_{2} + 6a_{3})+z^{2}(a_{2} +6a_{3} + 12a_{4})+z^{3}(a_{3} +8a_{4} + 20a_{5}) + ... = 0.\] This means that \[a_{n} + 2(n+1)a_{n+1} + (n^{2} + 3n + 2)a_{n+2} = 0.\] With \(a_{0} = 0\) and \(a_{1} = 2\), the rest of these terms may be recursively solved. \\

 

\end{document}